refactor and cleanup preorderTraversal somewhat

leetcode/preorderTraversal.dfy
@@ -1,185 +1,9 @@
 include "./invertTree.dfy"
-
+include "./preorderTraversalDefs.dfy"
 module PreorderTraversal {
     import opened InvertBinaryTree
     import Std.Collections.Seq
-    method SetToSeq<T>(s: set<T>) returns (xs: seq<T>)
-      ensures multiset(s) == multiset(xs)
-    {
-      xs := [];
-      var left: set<T> := s;
-      while left != {}
-        invariant multiset(left) + multiset(xs) == multiset(s)
-      {
-        var x :| x in left;
-        left := left - {x};
-        xs := xs + [x];
-      }
-    }
-
-    function toSet<T>(s: seq<T>): set<T> 
-      decreases |s|
-    {
-      if s == [] then {} else toSet(s[..|s|-1])+{s[|s|-1]}
-    }
-
-    function children(node: TreeNode): set<TreeNode> 
-        // requires node.Valid()
-        reads node
-        // ensures children(node) < node.repr
-        // ensures node !in children(node)
-    {
-        (if node.right != null then {node.right} else {}) + 
-        (if node.left != null then {node.left} else {})
-    }
-
-    lemma childrenLemma(node: TreeNode)
-        requires node.Valid()
-        ensures children(node) < node.repr
-        ensures node !in children(node)
-    {
-
-    }
-
-    function childStack(node: TreeNode?): seq<TreeNode> 
-        reads if node == null then {} else node.repr
-        requires node != null ==> node.Valid()
-        ensures forall x :: x in childStack(node) ==> x.Valid()
-    {
-        if node == null then [] else
-        (if node.right != null then 
-        assert node.Valid();
-        assert node.right.Valid();
-        [node.right] else []) + 
-        (if node.left != null then
-        assert node.Valid();
-        assert node.left.Valid();
-         [node.left] else [])
-    }
-
-    function rightStack(node: TreeNode): seq<TreeNode> 
-        reads node
-        // requires node.Valid()
-    {
-      if node.right != null then [node.right] else []
-    }
-
-    function rightStackUnvisited(node: TreeNode, visited: set<TreeNode>): seq<TreeNode> 
-        reads node
-        // requires node.Valid()
-    {
-      if node.right != null && node.right !in visited then [node.right] else []
-    }
-
-    lemma rightStackUnvisitedLemma(node: TreeNode, visited: set<TreeNode>)
-      ensures rightStackUnvisited(node, visited) != [] ==> |rightStackUnvisited(node, visited)| == 1
-    {
-
-    }
-
-    predicate leftStackVisited(node: TreeNode, visited: set<TreeNode>) 
-      reads node
-    {
-      if node.left != null then node.left in visited else true
-    }
-
-    lemma childStackLemma(node: TreeNode?)
-        requires node != null ==> node.Valid()
-        ensures node == null ==> childStack(node) == []
-        ensures node != null && node.left == null && node.right == null ==> childStack(node) == []
-        ensures node != null && node.left != null && node.right == null ==> childStack(node) == [node.left]
-        ensures node != null && node.left == null && node.right != null ==> childStack(node) == [node.right]
-        ensures node != null && node.left != null && node.right != null ==> childStack(node) == [node.right, node.left]
-        ensures node != null ==> TreeUnion(childStack(node)) == node.repr-{node}
-      {
-        if node == null {
-
-        } else{
-          if node.right != null && node.left != null {
-              assert node.right.repr + node.left.repr == node.repr - {node};
-              TreeUnionConcat([node.right],[ node.left]);
-              assert TreeUnion(childStack(node)) == node.right.repr + node.left.repr;
-            } else if node.right != null && node.left == null {
-            } else if node.right == null && node.left != null {
-            }else {
-            }
-        }
-      }
-
-    function mapNodes(ss: seq<TreeNode>): seq<int> 
-        reads set i | 0 <= i < |ss| :: ss[i]
-    {
-        if ss == [] then [] else [ss[0].val]+mapNodes(ss[1..])
-    }    
-
-    function parentStack(node: TreeNode): seq<TreeNode> 
-      reads node, node.repr
-      requires node.Valid()
-    {
-      if |childStack(node)| > 0 then [node] else []
-    }
-
-    lemma parentStackLemma(node: TreeNode)
-      requires node.Valid()
-      ensures forall x :: x in parentStack(node) ==> x.Valid()
-    {
-
-    }
-
-    // ghost function AllReprs(ss: seq<TreeNode>): set<TreeNode>
-    //   reads ss, ss[0]
-    // {
-    //   if ss == []  then {} else ss[0].repr + AllReprs(ss[1..])
-    // }
-
-    function setUnion<T>(xs: seq<set<T>>): set<T> {
-      if xs == [] then {} else xs[0] + setUnion(xs[1..])
-    }
-
-    function reprUnion(xs: seq<TreeNode>): set<TreeNode> 
-      reads xs
-      ensures forall x :: x in xs ==> x.repr <= reprUnion(xs)
-    {
-      if xs == [] then {} else xs[0].repr + reprUnion(xs[1..])
-    }
-
-    function pruneParents(ss: seq<TreeNode>, visited: set<TreeNode>): seq<TreeNode> 
-      // reads (set i | 0 <= i < |ss| :: ss[i]) + setUnion(Seq.Map((x: TreeNode) reads x => x.repr, ss))
-      reads (set i | 0 <= i < |ss| :: ss[i])
-        // reads AllReprs(ss)
-        // reads ss
-        // requires forall x :: x in ss ==> x.Valid()
-        ensures forall x :: x in pruneParents(ss, visited) ==> x in ss
-    {
-      if ss != [] then if children(ss[|ss|-1]) <= visited then pruneParents(ss[..|ss|-1], visited) else ss else []
-    }
-
-    lemma pruneParentsLemma(ss: seq<TreeNode>, visited: set<TreeNode>)
-      requires AllAncestors(ss)
-      ensures AllAncestors(pruneParents(ss, visited))
-    {
-
-    }
-
-    lemma pruneParentsLemma2(ss: seq<TreeNode>, visited: set<TreeNode>)
-      requires AllAncestors(ss)
-      requires ss!=[]
-      requires pruneParents(ss, visited) == []
-      ensures forall x: TreeNode :: x in ss && x !in pruneParents(ss, visited) ==> children(x) <= visited
-    {
-      if ss == [] {
-
-      }else if |ss| == 1 {
-        assert ss[0] in ss;
-        if children(ss[0])<= visited {
-          assert ss[0] !in  pruneParents(ss, visited);
-        }else{
-          assert ss[0] in  pruneParents(ss, visited);
-        }
-      }else{
-
-      }
-    }
+    import opened PreorderTraversalSupp
 
     lemma newStackNotEmptyImpliesParentsNotEmpty(parents: seq<TreeNode>, stack: seq<TreeNode>, visited: set<TreeNode>, unvisited: set<TreeNode>)
       requires allLeftVisited(parents, visited)
@@ -217,7 +41,7 @@ module PreorderTraversal {
       requires AllDisjoint(stack)
       requires unvisited == TreeUnion(stack)
       requires pruneParents(parents+parentStack(stack[|stack|-1]), visited+{stack[|stack|-1]}) == []
-      // requires allLeftVisited(parents, visited)
+      requires allLeftVisited(parents, visited)
       requires stack == allRight(parents, visited)
       ensures stack[..|stack|-1]+childStack(stack[|stack|-1]) == []
 
@@ -280,207 +104,7 @@ module PreorderTraversal {
         assert stack[..|stack|-1]+childStack(stack[|stack|-1]) == [];
     }
 
-  predicate compare(a: TreeNode, b: TreeNode)
-    reads a, b
-  {
-    a.val <= b.val
-  }
-
-  predicate AllAncestors(ts: seq<TreeNode>) 
-      reads set i | 0 <= i < |ts| :: ts[i]
-  {
-    forall i :: 0 <= i < |ts|-1 ==> childOf(ts[i+1], ts[i])
-  }
-
-  lemma AllAncestorsLemma(ts: seq<TreeNode>, i: int, j : int)
-    requires forall x :: x in ts ==> x.Valid()
-    requires AllAncestors(ts)
-    requires 0 <=i < j < |ts|
-    ensures ts[j].repr < ts[i].repr
-    ensures ts[j] in ts[i].repr
-  {
-    // assert childOf(ts[j], ts[j-1]);
-    assert ts[j-1] in ts;
-    assert ts[j] in ts[j-1].repr;
-    if j-1 > i {
-
-    AllAncestorsLemma(ts, i, j-1);
-    assert ts[j-1] in ts;
-    // assert ts[j-1].repr
-    }else{
-
-    }
-  }
-
-  predicate AllAncestorsDesc(ts: seq<TreeNode>) 
-      reads set i | 0 <= i < |ts| :: ts[i], reprUnion(ts), set i | 0 <= i < |ts| :: ts[i].left, set i | 0 <= i < |ts| :: ts[i].right
-  {
-    forall i :: 0 <= i < |ts|-1 ==> childOf(ts[i+1], ts[i]) || descOf(ts[i+1], ts[i])
-  }
-
-  predicate childOf(a: TreeNode, b: TreeNode)
-    reads a,b
-  {
-    a == b.left || a == b.right
-  }
-
-  predicate descOf(a: TreeNode, b: TreeNode)
-    reads a,b,b.repr, if b.left != null then {b.left} else {}, if b.right != null then {b.right} else {}
-  {
-    (b.left != null && a in b.left.repr) || (b.right != null && a in b.right.repr)
-  }
-
-lemma ThereIsAMinimum(s: set<TreeNode>)
-  requires s != {}
-  ensures exists x :: x in s && forall y :: y in s ==> compare(x, y)
-{
-  var x :| x in s;
-  if s == {x} {
-    // obviously, x is the minimum
-  } else {
-    // The minimum in s might be x, or it might be the minimum
-    // in s - {x}. If we knew the minimum of the latter, then
-    // we could compare the two.
-    // Let's start by giving a name to the smaller set:
-    var s' := s - {x};
-    // So, s is the union of s' and {x}:
-    assert s == s' + {x};
-    // The following lemma call establishes that there is a
-    // minimum in s'.
-    ThereIsAMinimum(s');
-  }
-}
-
-// lemma ThereIsAMinimumTwo(s: set<int>)
-//   requires s != {}
-//   ensures exists x :: x in s && forall y :: y in s ==> x <= y
-// {
-//   var x :| x in s;
-//   if s == {x} {
-//   } else {
-//     var s' := s - {x};
-//     assert s == s' + {x};
-//     ThereIsAMinimumTwo(s');
-//   }
-// }
-
-//     ghost function gmapNodeSet(ss: set<TreeNode>): set<int> 
-//         reads ss
-//         ensures forall xx :: xx in gmapNodeSet(ss) ==> exists s :: s in ss && s.val == xx
-//     {
-//         if ss == {} then 
-//             {}
-//         else 
-//             var s :| s in ss;
-//             {s.val}+gmapNodeSet(ss - {s})
-//     }    
-
-// lemma ThereIsAMinimumG(s: set<TreeNode>)
-//   requires s != {}
-//   ensures exists x :: x in gmapNodeSet(s) && forall y :: y in gmapNodeSet(s) ==> x<= y
-// {
-//     var xx :| xx in s  && gmapNodeSet(s) == {xx.val}+gmapNodeSet(s-{xx});
-//     var x :| x in gmapNodeSet(s) && xx.val == x;
-//   if s == {xx} {
-//     // obviously, x is the minimum
-//   } else {
-//     var s' := s - {xx};
-//     assert s == s' + {xx};
-//     ThereIsAMinimumG(s');
-//     var mm :| mm in gmapNodeSet(s') && forall y :: y in gmapNodeSet(s') ==> mm <= y;
-//     if x <= mm {
-//       assert x in gmapNodeSet(s) && forall y :: y in gmapNodeSet(s) ==> x <= y;
-//     }else{
-//       assert mm in gmapNodeSet(s) && forall y :: y in gmapNodeSet(s) ==> mm <= y;
-        
-//     }
-//   }
-// }
-
-    predicate uniqueNodes(ss: set<TreeNode>)
-      reads ss
-    {
-      forall x,y :: x in ss && y in ss && x != y ==> x.val != y.val 
-    }
-
-    ghost predicate AllDisjoint(ts: seq<TreeNode>)
-        reads set x | 0 <= x < |ts| :: ts[x]
-    {
-        forall x, y :: 0 <= x < y < |ts| && x != y ==> ts[x].repr !! ts[y].repr
-    }
-
-  
-
-    lemma  AllDisjointMaint(stack: seq<TreeNode>, current: TreeNode)
-        requires |stack| > 0
-        requires AllDisjoint(stack)
-        requires forall x :: x in stack ==> x.Valid()
-        requires current == stack[|stack|-1]
-        ensures current.left != null && current.right != null ==> AllDisjoint(stack[..|stack|-1]+[current.right, current.left])
-        ensures current.left != null && current.right == null ==> AllDisjoint(stack[..|stack|-1]+[current.left])
-        ensures current.left == null && current.right != null ==> AllDisjoint(stack[..|stack|-1]+[current.right])
-        ensures current.left == null && current.right == null ==> AllDisjoint(stack[..|stack|-1])
-    {
-            assert current.Valid();
-            if current.right != null && current.left != null {
-                // assert AllDisjoint(stack[..|stack|-1]+[current.right, current.left]);
-            } else if current.right != null && current.left == null {
-                assert current.right.repr < current.repr;
-                // assert AllDisjoint(stack[..|stack|-1]+[current.right]);
-            } else if current.right == null && current.left != null {
-                // assert AllDisjoint(stack[..|stack|-1]+[current.left]);
-            }else {
-                // assert AllDisjoint(stack[..|stack|-1]);
-            }
-    }
-
-    lemma TreeUnionMaint(stack: seq<TreeNode>, current: TreeNode, unvisited: set<TreeNode>)
-        requires |stack| > 0
-        requires unvisited == TreeUnion(stack)
-        requires AllDisjoint(stack)
-        requires forall x :: x in stack ==> x.Valid()
-        requires current == stack[|stack|-1]
-        ensures TreeUnion(stack[..|stack|-1]+childStack(current)) == unvisited-{current}
-    {
-        childStackLemma(current);
-        assert current in stack;
-        // assert current.Valid();
-        assert stack == stack[..|stack|-1]+[stack[|stack|-1]];
-        TreeUnionConcat(stack[..|stack|-1],[stack[|stack|-1]]);
-        // assert TreeUnion(stack) == TreeUnion(stack[..|stack|-1])+TreeUnion([stack[|stack|-1]]);
-        assert TreeUnion([stack[|stack|-1]]) == current.repr;
-        assert TreeUnion(stack[..|stack|-1]) !! current.repr by {
-            forall x | x in TreeUnion(stack[..|stack|-1])
-                ensures x !in current.repr
-            {
-                // var xx :| xx in stack[..|stack|-1] && x in xx.repr;
-                TreeUnionLemma(stack[..|stack|-1]);
-                var k :| 0 <= k < |stack[..|stack|-1]| && x in stack[..|stack|-1][k].repr;
-                assert stack[..|stack|-1][k].repr !! current.repr;
-            }
-        }
-        // assert TreeUnion(stack[..|stack|-1]) == unvisited-current.repr;
-        if current.left != null && current.right != null {
-            assert current.right.repr + current.left.repr + {current} == current.repr;
-            assert current.right.repr + current.left.repr == current.repr - {current};
-            TreeUnionConcat([current.right],[current.left]);
-            // assert TreeUnion([current.right, current.left]) == current.right.repr + current.left.repr;
-            TreeUnionConcat(stack[..|stack|-1], [current.right, current.left]);
-        } else if current.left != null && current.right == null {
-            assert current.left.repr == current.repr - {current};
-            TreeUnionConcat(stack[..|stack|-1], [current.left]);
-            
-        }else if current.left == null && current.right != null {
-            assert current.right.repr == current.repr - {current};
-            TreeUnionConcat(stack[..|stack|-1], [current.right]);
-
-        }else if current.left == null && current.right == null {
-            TreeUnionConcat(stack[..|stack|-1], []);
-
-        }
-    }
-
-    lemma {:verify } {:vcs_split_on_every_assert} FlatMapVisitedARN(stack: seq<TreeNode>, parents: seq<TreeNode>, visited: set<TreeNode>, unvisited: set<TreeNode>, current: TreeNode, newStack: seq<TreeNode>, newParents: seq<TreeNode>)
+    lemma {:verify false} {:vcs_split_on_every_assert} FlatMapVisitedARN(stack: seq<TreeNode>, parents: seq<TreeNode>, visited: set<TreeNode>, unvisited: set<TreeNode>, current: TreeNode, newStack: seq<TreeNode>, newParents: seq<TreeNode>)
       requires |stack| > 0 
       requires current == stack[|stack|-1]
       requires current !in visited
@@ -579,7 +203,7 @@ lemma ThereIsAMinimum(s: set<TreeNode>)
       assert newStack == stack[..|stack|-1];
       assert stack[ |stack| - 1] == parents[ |parents| -1].right;
       if newStack == [] {
-      assume newParents == [];
+      assume {:axiom} newParents == [];
       assert newStack  == allRight(newParents, visited+{current});
       assert allLeftVisited(newParents, visited+{current});
 
@@ -909,107 +533,8 @@ lemma ThereIsAMinimum(s: set<TreeNode>)
       }
     }
 
-    predicate stackPred(stack: seq<TreeNode>, parents: seq<TreeNode>) 
-      reads parents, set i | 0 <= i < |parents| :: parents[i], reprUnion(parents)
-      requires forall parent :: parent in parents ==> parent.Valid()
-    {
-      stack == Seq.Flatten(Seq.Map(rightStack, parents)) || (|parents| > 0 && stack == Seq.Flatten(Seq.Map(rightStack, parents[..|parents|-1]))+childStack(parents[|parents|-1]))
-    }
 
-    function allRight(parents: seq<TreeNode>, visited: set<TreeNode>): seq<TreeNode> 
-      reads parents, set i | 0 <= i < |parents| :: parents[i], reprUnion(parents)
-    {
-      var visitMap := (x: TreeNode) reads x => rightStackUnvisited(x, visited);
-      Seq.Flatten(Seq.Map(visitMap, parents))
-    }
 
-    lemma flattenLemma<T>(xs: seq<seq<T>>, x: T)
-      requires x in Seq.Flatten(xs)
-      ensures x in Seq.Flatten(xs) ==> exists xx :: xx in xs && x in xx
-    {
-      if |xs| == 1 {
-        assert xs[0] in xs;
-        if x in xs[0] {
-
-        }else {
-          assert x !in xs[0];
-          assert x in Seq.Flatten(xs);
-          assert xs[1..] == [];
-          assert Seq.Flatten(xs) == xs[0];
-          assert false;
-        }
-      }else{
-        assert xs == [xs[0]] + xs[1..];
-        Seq.LemmaFlattenConcat([xs[0]], xs[1..]);
-        if x in xs[0] {
-
-        }else {
-          flattenLemma(xs[1..], x);
-        }
-
-      }
-    }
-
-    lemma allRightLemma(parents: seq<TreeNode>, visited: set<TreeNode>)
-      ensures forall x :: x in allRight(parents, visited) ==> exists i :: 0 <= i < |parents| && x in rightStackUnvisited(parents[i], visited)
-    {
-      forall x | x in allRight(parents, visited)
-        ensures exists i :: 0 <= i < |parents| && x in rightStackUnvisited(parents[i], visited)
-      {
-      var visitMap := (x: TreeNode) reads x => rightStackUnvisited(x, visited);
-        assert forall  k :: 0 <= k < |parents| ==> Seq.Map(visitMap, parents)[k] == rightStackUnvisited(parents[k], visited);
-        flattenLemma(Seq.Map(visitMap, parents), x);
-      }
-    }
-
-    function allRightPlusChildren(parents: seq<TreeNode>, visited: set<TreeNode>): seq<TreeNode>
-      reads parents, set i | 0 <= i < |parents| :: parents[i], reprUnion(parents)
-      requires |parents| > 0
-      requires forall parent :: parent in parents ==> parent.Valid()
-    {
-      var visitMap := (x: TreeNode) reads x => rightStackUnvisited(x, visited);
-      Seq.Flatten(Seq.Map(visitMap, parents[..|parents|-1]))+childStack(parents[|parents|-1])
-    }
-
-    lemma allRightPlusChildrenLemma(parents: seq<TreeNode>, visited: set<TreeNode>)
-      requires |parents| > 0
-      requires forall parent :: parent in parents ==> parent.Valid()
-      ensures forall x :: x in allRightPlusChildren(parents, visited) ==> exists i :: 0 <= i < |parents| && x in children(parents[i])
-    {
-      forall x | x in allRightPlusChildren(parents, visited)
-        ensures exists i :: 0 <= i < |parents| && x in children(parents[i])
-      {
-        //Seq.Flatten(Seq.Map(visitMap, parents[..|parents|-1]))+childStack(parents[|parents|-1])
-        var visitMap := (x: TreeNode) reads x => rightStackUnvisited(x, visited);
-        if x in Seq.Flatten(Seq.Map(visitMap, parents[..|parents|-1])) {
-        allRightLemma(parents[..|parents|-1], visited);
-        assert forall x :: x in allRight(parents[..|parents|-1], visited) ==> exists k :: 0 <= k < |parents[..|parents|-1]| && x in rightStackUnvisited(parents[..|parents|-1][k], visited);
-        }else{
-          assert x in childStack(parents[|parents|-1]);
-          assert x in children(parents[|parents|-1]);
-        }
-      }
-    }
-
-    predicate allLeftVisited(parents: seq<TreeNode>, visited: set<TreeNode>) 
-      reads parents, set i | 0 <= i < |parents| :: parents[i]
-    {
-      forall p :: p in parents ==> leftStackVisited(p, visited)
-    }
-
-    predicate allLeftReprVisited(parents: seq<TreeNode>, visited: set<TreeNode>) 
-      reads parents, set i | 0 <= i < |parents| :: parents[i], set i | 0 <= i < |parents| :: parents[i].left
-    {
-      forall p :: p in parents ==> forall c :: c in (if p.left != null then p.left.repr else {}) ==> c in visited
-    }
-
-    predicate stackPred2(stack: seq<TreeNode>, parents: seq<TreeNode>, visited: set<TreeNode>) 
-      reads parents, set i | 0 <= i < |parents| :: parents[i], reprUnion(parents)
-      requires forall parent :: parent in parents ==> parent.Valid()
-    {
-      (stack == allRight(parents, visited) && allLeftVisited(parents, visited))
-      || (|parents| > 0 && stack == allRightPlusChildren(parents, visited) && allLeftVisited(parents[..|parents|-1], visited))
-    }
 
     /**
       This is the main algorithm I am trying to verify as iteratively equivalent to PreorderTraversal. 
@@ -1154,6 +679,9 @@ lemma ThereIsAMinimum(s: set<TreeNode>)
             invariant unvisited == TreeUnion(stack)
             /*verifies */
             invariant 0 <= i <= |pro|
+            invariant parents != [] ==> stack != []
+
+            invariant parents != [] ==> childOf(stack[ |stack| -1], parents[ |parents| -1])
             // invariant result == pro[..i]
             // invariant |stack| > 0 && i < |pro| ==> stack[|stack|-1] == pro[i]
             decreases |root.repr| - i
@@ -1229,6 +757,7 @@ lemma ThereIsAMinimum(s: set<TreeNode>)
             print "post ", "parentIndices ", parentIndices, " \n";
             expect parents != [] ==> stackPred2(stack, parents, visited), "After pred works";
             expect AllAncestors(parents), "after stack AllAncestors true";
+            // parentsEmptyImplyStackEmpty(parents, stack, visited, unvisited);
             i := i + 1;
         }
         assert result == PreorderTraversal(root)[0..|PreorderTraversal(root)|];
